Use shared expressions when performing CE

Proofs/Rewrites.thy
@@ -48,9 +48,144 @@ fun bool_to_val_width1 :: "bool \<Rightarrow> Value" where
 
 fun constantCondition :: "bool \<Rightarrow> ID \<Rightarrow> IRNode \<Rightarrow> IRGraph \<Rightarrow> IRGraph" where
   "constantCondition val nid (IfNode cond t f) g = 
-    replace_node nid (IfNode (nextNid g) t f, stamp g nid) 
-      (add_node (nextNid g) ((ConstantNode (bool_to_val_width1 val)), constantAsStamp (bool_to_val_width1 val)) g)" |
+    (let (g', nid') = Predicate.the (unrepE g (ConstantExpr (bool_to_val_width1 val))) in
+      replace_node nid (IfNode nid' t f, stamp g nid) g')" |
   "constantCondition cond nid _ g = g"
+
+inductive_cases unrepUnaryE:
+  "unrep g (UnaryExpr op e) (g', nid)"
+inductive_cases unrepBinaryE:
+  "unrep g (BinaryExpr op e1 e2) (g', nid)"
+inductive_cases unrepConditionalE:
+  "unrep g (ConditionalExpr c t f) (g', nid)"
+inductive_cases unrepParamE:
+  "unrep g (ParameterExpr i s) (g', nid)"
+inductive_cases unrepConstE:
+  "unrep g (ConstantExpr c) (g', nid)"
+inductive_cases unrepLeafE:
+  "unrep g (LeafExpr n s) (g', nid)"
+inductive_cases unrepVariableE:
+  "unrep g (VariableExpr v s) (g', nid)"
+inductive_cases unrepConstVarE:
+  "unrep g (ConstantVar c) (g', nid)"
+
+lemma unrepDet:
+  assumes "unrep g e (g'\<^sub>1, nid\<^sub>1)"
+  assumes "unrep g e (g'\<^sub>2, nid\<^sub>2)"
+  shows "g'\<^sub>1 = g'\<^sub>2 \<and> nid\<^sub>1 = nid\<^sub>2"
+  using assms proof (induction e arbitrary: g g'\<^sub>1 nid\<^sub>1 g'\<^sub>2 nid\<^sub>2)
+  case (UnaryExpr op e)
+  then obtain g' x where "g \<oplus> e \<leadsto> (g', x)"
+    by (meson unrepUnaryE)
+  then have "\<forall>gg xx. g \<oplus> e \<leadsto> (gg, xx) \<longrightarrow> g' = gg \<and> x = xx"
+    by (simp add: UnaryExpr.IH)
+  then show ?case
+    by (smt (verit, best) UnaryExpr.prems(1) UnaryExpr.prems(2) option.discI option.inject unrepUnaryE)
+next
+  case (BinaryExpr x1 e1 e2)
+  then show ?case
+    by (smt (verit) option.distinct(1) option.inject unrepBinaryE)
+next
+  case (ConditionalExpr e1 e2 e3)
+  then show ?case 
+    by (smt (verit) option.distinct(1) option.inject unrepConditionalE)
+next
+  case (ParameterExpr x1 x2)
+  then show ?case
+    by (smt (verit) option.distinct(1) option.inject unrepParamE)
+next
+  case (LeafExpr x1 x2)
+  then show ?case 
+    by (smt (verit) option.distinct(1) option.inject unrepLeafE)
+next
+  case (ConstantExpr x)
+  then show ?case
+    by (smt (verit) option.distinct(1) option.inject unrepConstE)
+next
+  case (ConstantVar x)
+  then show ?case
+    by (smt (verit) option.distinct(1) option.inject unrepConstVarE)
+next
+  case (VariableExpr x1 x2)
+  then show ?case
+    by (smt (verit) option.distinct(1) option.inject unrepVariableE)
+qed
+
+
+lemma unwrapUnrepE:
+  assumes "unrep g e (g', nid')"
+  shows "(g', nid') = Predicate.the (unrepE g e)"
+  using assms unrepEI unrepDet unfolding Predicate.the_def
+  by (metis eval_usages.cases pred.sel the_equality unrepE_def)
+
+lemma constantCondition_sem:
+  assumes "(unrep g (ConstantExpr (bool_to_val_width1 val)) (g', nid'))"
+  shows "constantCondition val nid (IfNode cond t f) g =
+    replace_node nid (IfNode nid' t f, stamp g nid) g'"
+  using assms unfolding constantCondition.simps
+  using unwrapUnrepE by auto
+
+fun wf_insert :: "IRGraph \<Rightarrow> IRExpr \<Rightarrow> bool" where
+  "wf_insert g (LeafExpr n s) = is_preevaluated (kind g n)" |
+  "wf_insert g (VariableExpr v s) = False" |
+  "wf_insert g (ConstantVar v) = False" |
+  "wf_insert g _ = True"
+
+(*
+lemma
+  assumes "wf_insert g e"
+  shows "\<exists>g' nid'. unrep g e (g', nid')"
+  using assms proof (induction e arbitrary: g)
+    case (UnaryExpr op e)
+    then obtain g' x where "g \<oplus> e \<leadsto> (g', x)"
+      by blast
+    then show ?case 
+      apply (cases "find_node_and_stamp g' (unary_node op x, stamp_unary op (stamp g' x)) = Some n")
+      using UnaryNodeSame apply blast
+      by (meson UnaryNodeNew UnaryNodeSame not_Some_eq)
+  next
+    case (BinaryExpr op e1 e2)
+    then obtain g' x where "g \<oplus> e1 \<leadsto> (g', x)"
+      by blast
+    also obtain g'' y where "g' \<oplus> e2 \<leadsto> (g'', y)"
+      using BinaryExpr.IH(2) by force
+    then show ?case 
+      apply (cases "find_node_and_stamp g'' (bin_node op x y, stamp_binary op (stamp g'' x) (stamp g'' y)) = Some n")
+      using BinaryNodeSame calculation apply blast
+      by (meson BinaryNodeNew BinaryNodeSame calculation not_Some_eq)
+  next
+    case (ConditionalExpr e1 e2 e3)
+    then obtain g' x where "g \<oplus> e1 \<leadsto> (g', x)"
+      by blast
+    also obtain g'' y where "g' \<oplus> e2 \<leadsto> (g'', y)"
+      using ConditionalExpr.IH(2) by force
+    moreover obtain g''' z where "g'' \<oplus> e3 \<leadsto> (g''', z)"
+      using ConditionalExpr.IH(3) by force
+    ultimately show ?case 
+      by (meson option.exhaust_sel unrep.intros(5) unrep.intros(6))
+  next
+    case (ParameterExpr x1 x2)
+    then show ?case
+      by (meson option.exhaust_sel unrep.intros(3) unrep.intros(4))
+  next
+    case (LeafExpr x1 x2)
+    then show ?case using assms sledgehammer
+  next
+    case (ConstantExpr x)
+    then show ?case
+      by (meson not_Some_eq unrep.intros(1) unrep.intros(2))
+  next
+    case (ConstantVar x)
+    then show ?case sorry
+  next
+    case (VariableExpr x1 x2)
+    then show ?case sledgehammer
+  qed
+*)
+
+lemma insertConst:
+  "\<exists>g' nid'. unrep g (ConstantExpr c) (g', nid')"
+  by (meson not_None_eq unrep.intros(1) unrep.intros(2))
 
 lemma constantConditionTrue:
   assumes "kind g ifcond = IfNode cond t f"
@@ -59,27 +194,38 @@ lemma constantConditionTrue:
 proof -
   have ifn: "\<And> c t f. IfNode c t f \<noteq> NoNode"
     by simp
-  then have if': "kind g' ifcond = IfNode (nextNid g) t f"
-    using assms constantCondition.simps(1) replace_node_lookup by presburger
+  obtain g'' nid' where unrep: "unrep g (ConstantExpr (bool_to_val_width1 True)) (g'', nid')"
+    using insertConst by blast
+  then have "kind g'' nid' = ConstantNode (bool_to_val_width1 True)"
+    by (smt (verit) ConstUnrepE IRExpr.simps(18) IRExpr.simps(30) IRExpr.simps(40) IRExpr.simps(48) IRExpr.simps(54) IRExpr.simps(6) IRNode.simps(1141) find_exists_kind find_new_kind option.distinct(1) option.inject unrep.simps)
+  also have "nid' \<noteq> ifcond"
+    by (smt (verit) IRExpr.simps(18) IRExpr.simps(30) IRExpr.simps(40) IRNode.distinct(981) \<open>g::IRGraph \<oplus> ConstantExpr (bool_to_val_width1 True) \<leadsto> (g''::IRGraph, nid'::nat)\<close> assms(1) calculation fresh_ids ifn not_in_g prod.inject unrep.simps)
+  moreover have "g' = replace_node ifcond (IfNode nid' t f, stamp g ifcond) g''"
+    using assms constantCondition_sem unrep by presburger
+  moreover have "kind g' nid' = ConstantNode (bool_to_val_width1 True)"
+    using assms constantCondition.simps(1) replace_node_unchanged 
+    by (metis DiffI calculation(1) calculation(2) calculation(3) emptyE insert_iff unrep unrep_contains)
+  moreover have if': "kind g' ifcond = IfNode nid' t f"
+    using ifn assms constantCondition.simps(1) replace_node_lookup
+    using calculation(3) by blast
   have truedef: "bool_to_val True = (IntVal 32 1)"
     by auto
   from ifn have "ifcond \<noteq> (nextNid g)"
     by (metis assms(1) emptyE ids_some nextNidNotIn)
   moreover have "\<And> c. ConstantNode c \<noteq> NoNode"
     by simp
-  ultimately have "kind g' (nextNid g) = ConstantNode (bool_to_val_width1 True)"
+  ultimately have "kind g' nid' = ConstantNode (bool_to_val_width1 True)"
     using add_changed
-    by (smt (z3) find_new_kind replace_node_unchanged singletonD replace_node_def not_in_g assms
-        other_node_unchanged constantCondition.simps(1) add_node_def)
-  then have c': "kind g' (nextNid g) = ConstantNode (IntVal 1 1)"
+    by fastforce
+  then have c': "kind g' nid' = ConstantNode (IntVal 1 1)"
     by simp
   have "valid_value (IntVal 1 1) (constantAsStamp (IntVal 1 1))"
     by fastforce
-  then have "[g', m, p] \<turnstile> nextNid g \<mapsto> IntVal 1 1"
-    using Value.distinct(1) \<open>kind g' (nextNid g) = ConstantNode (bool_to_val_width1 True)\<close>
+  then have "[g', m, p] \<turnstile> nid' \<mapsto> IntVal 1 1"
+    using Value.distinct(1) \<open>kind g' nid' = ConstantNode (bool_to_val_width1 True)\<close>
     by (metis bool_to_val_width1.simps(1) wf_value_def encodeeval_def ConstantExpr ConstantNode)
   from if' c' show ?thesis
-    by (metis (no_types, opaque_lifting) val_to_bool.simps(1) \<open>[g',m,p] \<turnstile> nextNid g \<mapsto> IntVal 1 1\<close>
+    by (metis (no_types, opaque_lifting) val_to_bool.simps(1) \<open>[g',m,p] \<turnstile> nid' \<mapsto> IntVal 1 1\<close>
         encodeeval_def zero_neq_one IfNode)
 qed
 
@@ -90,26 +236,30 @@ lemma constantConditionFalse:
 proof -
   have ifn: "\<And> c t f. IfNode c t f \<noteq> NoNode"
     by simp
-  then have if': "kind g' ifcond = IfNode (nextNid g) t f"
-    by (metis assms constantCondition.simps(1) replace_node_lookup)
+  obtain g'' nid' where unrep: "unrep g (ConstantExpr (bool_to_val_width1 False)) (g'', nid')"
+    using insertConst by blast
+  also have "kind g'' nid' = ConstantNode (bool_to_val_width1 False)"
+    by (smt (verit) IRExpr.sel(14) IRExpr.simps(18) IRExpr.simps(30) IRExpr.simps(40) IRExpr.simps(48) IRExpr.simps(54) IRNode.distinct(1077) find_exists_kind find_new_kind unrep unrep.simps unrepDet)
+  moreover have "nid' \<noteq> ifcond"
+    by (smt (verit) IRExpr.simps(18) IRExpr.simps(30) IRExpr.simps(40) IRNode.distinct(981) assms(1) calculation fresh_ids ifn not_in_g prod.inject unrep.simps)
+  moreover have "g' = replace_node ifcond (IfNode nid' t f, stamp g ifcond) g''"
+    using assms constantCondition_sem unrep by presburger
+  moreover have "kind g' nid' = ConstantNode (bool_to_val_width1 False)"
+    using assms constantCondition.simps(1) replace_node_unchanged 
+    by (metis DiffI calculation(2) calculation(3) calculation(4) emptyE insert_iff unrep unrep_contains)
+  moreover have if': "kind g' ifcond = IfNode nid' t f"
+    using ifn assms constantCondition.simps(1) replace_node_lookup
+    using calculation(4) by blast
   have falsedef: "bool_to_val False = (IntVal 32 0)"
     by auto
-  from ifn have "ifcond \<noteq> (nextNid g)"
-    by (metis assms(1) equals0D ids_some nextNidNotIn)
-  moreover have "\<And> c. ConstantNode c \<noteq> NoNode"
-    by simp
-  ultimately have "kind g' (nextNid g) = ConstantNode (bool_to_val_width1 False)"
-    by (smt (z3) add_changed add_node_def assms constantCondition.simps(1) find_new_kind not_in_g
-        other_node_unchanged replace_node_def singletonD)
-  then have c': "kind g' (nextNid g) = ConstantNode (IntVal 1 0)"
-    by simp
+  then have c': "kind g' nid' = ConstantNode (IntVal 1 0)"
+    by (simp add: calculation(5))
   have "valid_value (IntVal 1 0) (constantAsStamp (IntVal 1 0))"
     by auto
-  then have "[g', m, p] \<turnstile> nextNid g \<mapsto> IntVal 1 0"
+  then have "[g', m, p] \<turnstile> nid' \<mapsto> IntVal 1 0"
     by (meson ConstantExpr ConstantNode c' encodeeval_def wf_value_def)
   from if' c' show ?thesis
-    by (metis (no_types, opaque_lifting) val_to_bool.simps(1) \<open>[g',m,p] \<turnstile> nextNid g \<mapsto> IntVal 1 0\<close>
-        encodeeval_def IfNode)
+    by (meson IfNode \<open>[g'::IRGraph,m::nat \<Rightarrow> Value,p::Value list] \<turnstile> nid'::nat \<mapsto> IntVal (1::nat) (0::64 word)\<close> encodeeval_def val_to_bool.simps(1))
 qed
 
 lemma diff_forall:
@@ -137,12 +287,20 @@ lemma constantConditionNoEffect:
    apply (metis)
   by presburger+
 
-lemma constantConditionIfNode:
+(*lemma constantConditionIfNode:
   assumes "kind g nid = IfNode cond t f"
   shows "constantCondition val nid (kind g nid) g = 
     replace_node nid (IfNode (nextNid g) t f, stamp g nid) 
      (add_node (nextNid g) ((ConstantNode (bool_to_val_width1 val)), constantAsStamp (bool_to_val_width1 val)) g)"
-  by (simp add: assms)
+  by (simp add: assms)*)
+
+lemma changeonly_ConstantExpr:
+  assumes "unrep g (ConstantExpr c) (g', nid)"
+  shows "changeonly {} g g'"
+  using assms 
+  apply (cases "find_node_and_stamp g (ConstantNode c, constantAsStamp c) = None")
+  apply (smt (verit, del_insts) ConstantNodeNew add_changed changeonly.simps fresh_ids insertE unrepDet)
+  by (smt (verit) IRExpr.sel(14) IRExpr.simps(18) IRExpr.simps(30) IRExpr.simps(40) IRExpr.simps(48) changeonly.simps unrep.simps unrepDet)
 
 lemma constantCondition_changeonly:
   assumes "nid \<in> ids g"
@@ -150,11 +308,16 @@ lemma constantCondition_changeonly:
   shows "changeonly {nid} g g'"
 proof (cases "is_IfNode (kind g nid)")
   case True
-  have "nextNid g \<notin> ids g"
-    by (metis emptyE nextNidNotIn)
+  obtain g'' nid' where unrep: "unrep g (ConstantExpr (bool_to_val_width1 b)) (g'', nid')"
+    using insertConst by blast
+  also have "changeonly {} g g''"
+    using changeonly_ConstantExpr unrep by blast
+  moreover have "\<exists>t f ifcond. g' = replace_node nid (IfNode nid' t f, stamp g ifcond) g''"
+    using assms constantCondition_sem unrep
+    by (metis True is_IfNode_def)
   then show ?thesis
     using assms replace_node_changeonly add_node_changeonly unfolding changeonly.simps
-    by (metis (no_types, lifting) insert_iff is_IfNode_def constantCondition.simps(1) True)
+    by (metis calculation(2) changeonly.elims(2) empty_iff)
 next
   case False
   have "g = g'"
